Partial proofs of search and insert

bst.c
@@ -1,8 +1,8 @@
 #include <stddef.h>
 
-extern void * malloc(size_t n); // Why not include stdlib?
+extern void * malloc(size_t n);
+extern void * free(size_t n);
 
-// TODO: Generalize `int` to `void *` (will require a function pointer to compare elements for search)
 struct bst {
   int key;
   int val;
@@ -34,8 +34,6 @@ struct bst * search_bst(struct bst * bst, int key) {
 }
 
 void insert_bst(struct bst ** bst, int key, int val) {
-  // if (!bst) return; // Is this necessary? Don't we assume bst<>nullval in the spec? (Implicitly through the data_at).
-  // else
   for (;;) {
     if (!(*bst)) {
       *bst = new_bst(key, val);
@@ -52,7 +50,117 @@ void insert_bst(struct bst ** bst, int key, int val) {
   }
 }
 
-// TODO: Delete
+// Assumes a non-empty bst
+struct bst pop_min(struct bst ** bst_ptr);
+
+void delete_bst(struct bst ** parent_ptr, int key) {
+  struct bst * parent = *parent_ptr;
+  if (!parent)
+    return;
+  else if (key == parent->key) {
+    if (parent->left) {
+      if (parent->right) {
+        struct bst min = pop_min(&(parent->right));
+        parent->key = min.key;
+        parent->val = min.val;
+      }
+      else {
+        *parent_ptr = parent->left;
+        free(parent);
+      }
+    }
+    else {
+      if (parent->right) {
+        *parent_ptr = parent->right;
+        free(parent);
+      }
+      else {
+        free(parent);
+        *parent_ptr = (struct bst *)NULL;
+      }
+      // Move free(parent) to here?
+    }
+  }
+  else {
+    // invariant tip: key != parent->key
+    for (;;) {
+      if (key < parent->key) {
+        if (!(parent->left))
+          return;
+        else if (key == parent->left->key) {
+          if (parent->left->left) {
+            if (parent->left->right) {
+              struct bst min = pop_min(&(parent->left->right));
+              parent->left->key = min.key;
+              parent->left->val = min.val;
+              return;
+            }
+            else {
+              struct bst * del = parent->left;
+              parent->left = parent->left->left;
+              free(del);
+              return;
+            }
+          }
+          else {
+            if (parent->left->right) {
+              struct bst * del = parent->left;
+              parent->left = parent->left->right;
+              free(del);
+              return;
+            }
+            else {
+              free(parent->left);
+              parent->left = (struct bst *)NULL;
+              return;
+            }
+            // free(parent)
+          }
+          // return;
+        }
+        else 
+          parent = parent->left;
+      }
+      else {
+        if (!(parent->right))
+          return;
+        if (key == parent->right->key) {
+          if (parent->right->left) {
+            if (parent->right->right) {
+              struct bst min = pop_min(&(parent->right->right));
+              parent->right->key = min.key;
+              parent->right->val = min.val;
+              return;
+            }
+            else {
+              struct bst * del = parent->right;
+              parent->right = parent->right->left;
+              free(del);
+              return;
+            }
+          }
+          else {
+            if (parent->right->right) {
+              struct bst * del = parent->right;
+              parent->right = parent->right->right;
+              free(del);
+              return;
+            }
+            else {
+              free(parent->right);
+              parent->right = (struct bst *)NULL;
+              return;
+            }
+            // free(parent)
+          }
+          // return;
+        }
+        else 
+          parent = parent->right;
+     }
+    }
+  }
+}
 
 // TODO: Free
 
