Verif_bst.v
@@ -22,14 +22,29 @@ Arguments bin_tree _%type_scope.
 Arguments leaf {A}%type_scope.
 Arguments node {A}%type_scope.
 
+(* bin_tree with *exactly* one hole *)
 Inductive bin_tree_hole (A: Type) : Type :=
-  | hole  : bin_tree_hole A 
-  | hLeaf : bin_tree_hole A
-  | hNode : A -> bin_tree_hole A -> bin_tree_hole A -> bin_tree_hole A.
+  | hole : bin_tree_hole A
+  | node_hole_l : A -> bin_tree_hole A -> bin_tree A -> bin_tree_hole A
+  | node_hole_r : A -> bin_tree A -> bin_tree_hole A -> bin_tree_hole A.
 Arguments bin_tree_hole _%type_scope.
-Arguments hole  {A}%type_scope.
-Arguments hLeaf {A}%type_scope.
-Arguments hNode {A}%type_scope.
+Arguments hole {A}%type_scope.
+Arguments node_hole_l {A}%type_scope.
+Arguments node_hole_r {A}%type_scope.
+
+Fixpoint fill_hole {A} (outer: bin_tree_hole A) (inner: bin_tree A) : bin_tree A :=
+  match outer with 
+  | hole => inner
+  | node_hole_l a l r => node a (fill_hole l inner) r
+  | node_hole_r a l r => node a l (fill_hole r inner)
+  end.
+
+Fixpoint extend_hole {A} (outer inner: bin_tree_hole A) : bin_tree_hole A :=
+  match outer with 
+  | hole => inner
+  | node_hole_l a l r => node_hole_l a (extend_hole l inner) r
+  | node_hole_r a l r => node_hole_r a l (extend_hole r inner)
+  end.
 
 Inductive bin_tree_forall {A} : bin_tree A -> (A -> Prop) -> Prop :=
   | bin_tree_forall_leaf : forall p, bin_tree_forall leaf p 
@@ -126,6 +141,116 @@ Fixpoint search {A} (k: Z) (b: bst A) : bst A :=
       end 
   end.
 
+Lemma wo_node_eq {A} : forall k (v1 v2: A) l1 l2 r1 r2,
+  well_ordered (node (k,v1) l1 r1) ->
+  is_subtree (node (k,v2) l2 r2) (node (k,v1) l1 r1) ->
+  node (k,v1) l1 r1 = node (k,v2) l2 r2.
+Proof.
+  intros.
+  inversion H0; subst.
+  - reflexivity. 
+  - inversion H; subst. 
+    eapply subtree_forall in H3; [|eassumption].
+    inversion H3; subst.
+    simpl in H5. lia.
+  - inversion H; subst. 
+    eapply subtree_forall in H3; [|eassumption].
+    inversion H3; subst.
+    simpl in H5. lia.
+Qed.
+
+Lemma wo_subtree_left {A} : forall k1 k2 (v1 v2: A) l1 l2 r1 r2,
+  well_ordered (node (k1,v1) l1 r1) ->
+  is_subtree (node (k2,v2) l2 r2) (node (k1,v1) l1 r1) ->
+  k2 < k1 ->
+  is_subtree (node (k2,v2) l2 r2) l1.
+Proof.
+  intros.
+  inversion H0; subst.
+  - lia.
+  - assumption.
+  - inversion H; subst.
+    eapply subtree_forall in H4; [|eassumption].
+    inversion H4; subst.
+    simpl in H6. lia.
+Qed.
+
+Lemma wo_subtree_right {A} : forall k1 k2 (v1 v2: A) l1 l2 r1 r2,
+  well_ordered (node (k1,v1) l1 r1) ->
+  is_subtree (node (k2,v2) l2 r2) (node (k1,v1) l1 r1) ->
+  k2 > k1 ->
+  is_subtree (node (k2,v2) l2 r2) r1.
+Proof.
+  intros.
+  inversion H0; subst.
+  - lia.
+  - inversion H; subst.
+    eapply subtree_forall in H4; [|eassumption].
+    inversion H4; subst.
+    simpl in H6. lia.
+  - assumption.
+Qed.
+
+Theorem search_spec {A} : forall (b: bst A) k v l r,
+  well_ordered b ->
+  is_subtree (node (k,v) l r) b ->
+  search k b = node (k,v) l r.
+Proof.
+  intros.
+  induction b.
+  - inversion H0.
+  - inversion H; subst.
+    simplify_assumps.
+    simpl.
+    find_Z_compare_destruct.
+    + eapply wo_node_eq; assumption.
+    + apply IHb1.
+      eapply wo_subtree_left; eassumption.
+    + apply IHb2.
+      eapply wo_subtree_right; eassumption.
+Qed.
+
+(* This acts as a complement to search - where search returns the subtree, this returns the original tree,
+   but with a hole where the subtree used to be. *)
+Fixpoint search_make_hole {A} (k: Z) (b: bst A) : bst_hole A := 
+  match b with 
+  | leaf => hole
+  | node (k', v) l r => 
+      match k ?= k' with 
+      | Eq => hole
+      | Lt => node_hole_l (k', v) (search_make_hole k l) r
+      | Gt => node_hole_r (k', v) l (search_make_hole k r)
+      end 
+  end.
+
+Theorem fill_search_hole {A} : forall k (b: bst A),
+  fill_hole (search_make_hole k b) (search k b) = b.
+Proof.
+  intros k b.
+  induction b.
+  - reflexivity.
+  - simpl.
+    destruct_pair.
+    find_Z_compare_destruct; simpl.
+    + reflexivity.
+    + f_equal. assumption.
+    + f_equal. assumption.
+Qed.
+
+(* This does search and search_make_hole together *)
+Fixpoint split_bst_at {A} (k: Z) (b: bst A) : bst_hole A * bst A :=
+  match b with 
+  | leaf => (hole, leaf)
+  | node (k', v) l r =>
+      match k ?= k' with 
+      | Eq => (hole, b)
+      | Lt => let (outer, inner) := split_bst_at k l 
+              in (node_hole_l (k', v) outer r, inner)
+      | Gt => let (outer, inner) := split_bst_at k r 
+              in (node_hole_r (k', v) l outer, inner)
+      end 
+  end.
+
 Theorem search_is_subtree : forall {A} k (b sub: bst A),
   search k b = sub -> is_subtree sub b.
 Proof.
@@ -133,7 +258,7 @@ Proof.
   induction b; try destruct_pair; simpl; intro H.
   - subst. constructor.
   - find_Z_compare_destruct.
-    + subst. constructor.
+    + constructor.
     + apply is_subtree_left.
       apply IHb1.
       assumption.
@@ -162,7 +287,7 @@ Proof.
     unify_goal.
   - simpl. destruct_pair.
     find_Z_compare_destruct;
-    subst; simpl; rewrite Heqc; assumption + unify_goal.
+    simpl; rewrite Heqc; assumption + unify_goal.
 Qed.
 
 (* BST representations *)
@@ -180,19 +305,40 @@ Fixpoint bst_rep (b: bst Z) (p: val): mpred :=
         bst_rep r pr
   end.
 
-(* Check isptr. *)
-Function bst_hole_rep (b: bst_hole Z) (p: val): mpred :=
+Theorem generalize_node_rep : forall (p pl pr: val) k v l r,
+  (malloc_token Ews t_bst p *
+  data_at Ews t_bst (Vint (Int.repr k), (Vint (Int.repr v), (pl, pr))) p *
+  bst_rep l pl *
+  bst_rep r pr
+  |-- bst_rep (node (k,v) l r) p
+  )%logic.
+Proof.
+  intros.
+  expand bst_rep.
+  repeat EExists.
+  entailer!.
+Qed.
+
+Fixpoint bst_hole_rep (b: bst_hole Z) (p: val): mpred :=
   match b with 
-  (* | hole => !! (is_pointer_or_null p) && emp *)
   | hole => emp
-  | hLeaf => (!! (p = nullval)) && emp 
-  | hNode (k, v) l r =>
-      EX pl pr: val, 
+  | node_hole_l (k, v) l r =>
+      EX pl pr: val,
         malloc_token Ews t_bst p *
         data_at Ews t_bst (Vint (Int.repr k), (Vint (Int.repr v), (pl, pr))) p *
         bst_hole_rep l pl *
+        bst_rep r pr
+  | node_hole_r (k, v) l r =>
+      EX pl pr: val,
+        malloc_token Ews t_bst p *
+        data_at Ews t_bst (Vint (Int.repr k), (Vint (Int.repr v), (pl, pr))) p *
+        bst_rep l pl *
         bst_hole_rep r pr
   end.
+
+(* Definition bst_rep_w_ptr b head k sub := 
+  let (outer, inner) := split_bst_at k b
+  in (bst_hole_rep outer head * bst_rep inner sub)%logic. *)
 
 Lemma bst_rep_local_prop: forall b p,
   bst_rep b p |-- !! (is_pointer_or_null p /\ (p = nullval <-> b = leaf)).
@@ -217,32 +363,6 @@ Proof.
 Qed.
 Hint Resolve bst_rep_valid_pointer : valid_pointer. 
 
-(* Lemma bst_hole_rep_local_prop: forall b p,
-  bst_hole_rep b p |-- !! (is_pointer_or_null p).
-  (* bst_hole_rep b p |-- !! (is_pointer_or_null p /\ (p = nullval <-> (b = hole \/ b = hLeaf)). *)
-Proof.
-  intros b p. induction b; try solve [unfold bst_hole_rep; entailer!].
-  destruct a.
-  expand bst_hole_rep.
-  entailer.
-  entailer!.
-Qed.
-Hint Resolve bst_hole_rep_local_prop : saturate_local.
- *)
-(* Lemma bst_hole_rep_valid_pointer: forall b p,
-  bst_hole_rep b p |-- valid_pointer p.
-Proof. 
-  intros b p. induction b; expand bst_hole_rep.
-  - entailer!. 
-    destruct p; try entailer!; unfold is_pointer_or_null in PNp.
-    + destruct Archi.ptr64; entailer!.
-    + admit.
-  - entailer!.
-  - destruct a. entailer.
-Admitted.
-Hint Resolve bst_hole_rep_valid_pointer : valid_pointer. 
- *)
-
 (* Function specifications *) 
 
 Definition new_bst_spec: ident * funspec := DECLARE _new_bst
@@ -262,7 +382,8 @@ Definition insert_bst_spec: ident * funspec :=
   WITH bst_ptr: val, head: val, k: Z, v: Z, b: bst Z, gv: globals
   PRE [tptr (tptr t_bst), tint, tint]
     PROP (repable_signed k; repable_signed v;
-          bin_tree_forall b (fun n => repable_signed (fst n)))
+          bin_tree_forall b (fun n => repable_signed (fst n));
+          well_ordered b)
     PARAMS (bst_ptr; Vint (Int.repr k); Vint (Int.repr v)) GLOBALS (gv)
     SEP (data_at Ews (tptr t_bst) head bst_ptr;
          bst_rep b head;
@@ -275,21 +396,22 @@ Definition insert_bst_spec: ident * funspec :=
            bst_rep (insert k v b) new_bst;
            mem_mgr gv).
 
-(* This specification could be stronger. It does not prove that the bst is unchanged. *)
-Definition search_bst_spec: ident * funspec := 
+ Definition search_bst_spec: ident * funspec := 
   DECLARE _search_bst 
   WITH head: val, k: Z, b: bst Z, gv: globals 
   PRE [tptr t_bst, tint]
-    PROP (repable_signed k; bin_tree_forall b (fun n => repable_signed (fst n)))
+    PROP (repable_signed k;
+          bin_tree_forall b (fun n => repable_signed (fst n));
+          well_ordered b)
     PARAMS (head; Vint (Int.repr k)) GLOBALS (gv)
     SEP (bst_rep b head; mem_mgr gv)
   POST [tptr t_bst] 
-    EX vret, EX b2,
-      PROP () 
-      RETURN (vret) 
-      SEP (b2; bst_rep (search k b) vret; mem_mgr gv).
-      (* SEP (bst_hole_rep () head; bst_rep (search k b) vret; mem_mgr gv). *)
-
+    EX vret,
+      (* PROP (fill_hole (search k b) outer_b = b) *)
+      PROP ()
+      RETURN (vret)
+      SEP (bst_hole_rep (search_make_hole k b) head; bst_rep (search k b) vret; mem_mgr gv).
+ 
 Definition Gprog: funspecs := 
   ltac:(with_library prog [new_bst_spec; insert_bst_spec; search_bst_spec]).
 
@@ -305,6 +427,9 @@ Inductive search_path : Z -> bst Z -> bst Z -> Prop :=
       search_path k l b -> k < k' -> search_path k (node (k',v) l r) b
   | path_step_r : forall k k' v l r b,
       search_path k r b -> k > k' -> search_path k (node (k',v) l r) b.
+
+(* Definition search_path_rep (k: Z) (outer inner: bst Z) : mpred :=
+  !! (search_path k outer inner) && () *)
 
 (* This is the direction a path will actually grow in *)
 Lemma path_step_down_l : forall k head k' v l r,
@@ -350,6 +475,29 @@ Proof.
     reflexivity.
 Qed.
 
+(* Theorem search_path_fail_hole : forall k b,
+  search_path k b leaf -> search_make_hole k b = b.
+Proof.
+  intros k b H.
+  induction b.
+  - reflexivity.
+  - simpl.
+    destruct_pair.
+    find_Z_compare_destruct.
+    + find_contradiction.
+    + f_equal.
+      apply IHb1.
+      inversion H; subst.
+      * assumption.
+      * lia.
+    + f_equal.
+      apply IHb2.
+      inversion H; subst.
+      * lia.
+      * assumption.
+Qed.
+ *)
+
 Theorem search_path_success: forall k b v l r,
   search_path k b (node (k,v) l r) -> search k b = (node (k,v) l r).
 Proof.
@@ -386,78 +534,1039 @@ Proof.
   - apply is_subtree_right. assumption.
 Qed.
 
+Definition proper_subtree {A} (b1 b2: bin_tree A) := b1 <> b2 /\ is_subtree b1 b2.
+
+Ltac break_let :=
+  match goal with
+    | [ H : context [ (let (_,_) := ?X in _) ] |- _ ] => destruct X eqn:?
+    | [ |- context [ (let (_,_) := ?X in _) ] ] => destruct X eqn:?
+  end.
+
+(* Intended for when `search_path k outer inner` *)
+Definition bst_subtract_path k (outer inner: bst Z) : bst_hole Z :=
+  match inner with 
+  | leaf => search_make_hole k outer
+  | node (k',v) l r => search_make_hole k' outer 
+  end.
+
+Lemma bst_subtract_path_b_b : forall k b, bst_subtract_path k b b = hole.
+Proof.
+  intros.
+  destruct b.
+  - reflexivity.
+  - simpl.
+    break_let.
+    rewrite Z.compare_refl.
+    reflexivity.
+Qed.
+
+Theorem fill_hole_bst_subtract_path: forall k b sub,
+  well_ordered b ->
+  search_path k b sub ->
+  fill_hole (bst_subtract_path k b sub) sub = b.
+Proof.
+  intros k b sub H_wo H_path.
+  induction H_path.
+  - destruct b.
+    + reflexivity.
+    + simpl.
+      destruct_pair.
+      rewrite Z.compare_refl.
+      reflexivity.
+  - inversion H_wo; subst.
+    simplify_assumps.
+    destruct b.
+    + simpl.
+      rewrite Zaux.Zcompare_Lt by assumption.
+      simpl.
+      f_equal.
+      simpl in *.
+      assumption.
+    + simpl.
+      destruct_pair.
+      simpl in *.
+      apply search_path_is_subtree in H_path.
+      find_Z_compare_destruct.
+      * eapply subtree_forall in H_path; [|eassumption].
+        inversion H_path; subst.
+        simpl in *.
+        lia.
+      * simpl.
+        f_equal.
+        assumption.
+      * eapply subtree_forall in H_path; [|eapply H4].
+        inversion H_path; subst.
+        simpl in *.
+        lia.
+  - inversion H_wo; subst.
+    simplify_assumps.
+    destruct b.
+    + simpl.
+      rewrite Zaux.Zcompare_Gt by lia.
+      simpl.
+      f_equal.
+      simpl in *.
+      assumption.
+    + simpl.
+      destruct_pair.
+      simpl in *.
+      apply search_path_is_subtree in H_path.
+      find_Z_compare_destruct.
+      * eapply subtree_forall in H_path; [|eassumption].
+        inversion H_path; subst.
+        simpl in *.
+        lia.
+      * eapply subtree_forall in H_path; [|eapply H5].
+        inversion H_path; subst.
+        simpl in *.
+        lia.
+      * simpl.
+        f_equal.
+        assumption.
+Qed.
+
+Theorem is_subtree_up_left {A}: forall (a: A) l r b,
+  is_subtree (node a l r) b -> is_subtree l b.
+Proof.
+  intros.
+  dependent induction H.
+  - apply is_subtree_left. constructor.
+  - apply is_subtree_left.
+    eapply IHis_subtree.
+    reflexivity.
+  - apply is_subtree_right.
+    eapply IHis_subtree.
+    reflexivity.
+Qed.
+
+Theorem is_subtree_up_right {A}: forall (a: A) l r b,
+  is_subtree (node a l r) b -> is_subtree r b.
+Proof.
+  intros.
+  dependent induction H.
+  - apply is_subtree_right. constructor.
+  - apply is_subtree_left.
+    eapply IHis_subtree.
+    reflexivity.
+  - apply is_subtree_right.
+    eapply IHis_subtree.
+    reflexivity.
+Qed.
+
+(* Alternatively, base this on a "proper" search_path *)
+(* Theorem hole_rep_fuse_left2 : forall search_k k v l r k' v' l' r' (curr head pl pr: val),
+  well_ordered (node (k,v) l r) ->
+  search_path search_k (node (k,v) l r) (node (k',v') l' r') ->
+  search_k < k' ->
+  (node (k,v) l r = node (k',v') l' r' -> head = curr) ->
+    bst_hole_rep (bst_subtract_path k (node (k,v) l r) (node (k',v') l' r')) head *
+    malloc_token Ews t_bst curr *
+    data_at Ews t_bst (Vint (Int.repr k'), (Vint (Int.repr v'), (pl, pr))) curr *
+    bst_rep r' pr
+    |-- bst_hole_rep (bst_subtract_path search_k (node (k,v) l r) l') head.
+Proof.
+  intros search_k k v l r.
+  induction (node (k,v) l r).
+  - intros. inversion H0.
+  -
+    intros.
+    simpl.
+    destruct_pair.
+    find_Z_compare_destruct.
+    + apply search_path_is_subtree in H0.
+      apply wo_node_eq in H0; [|assumption].
+      inversion H0; subst.
+      simplify_assumps; subst.
+      simpl; cancel.
+      destruct l'.
+      * simpl.
+        rewrite Zaux.Zcompare_Lt by assumption.
+        simpl.
+        repeat EExists.
+        entailer!.
+      * simpl. 
+        destruct_pair.
+        rewrite Z.compare_refl.
+        rewrite Zaux.Zcompare_Lt.
+        -- simpl.
+           Exists pl pr.
+           entailer!.
+        -- inversion H; subst.
+           inversion H5; subst.
+           simpl in *; assumption.
+    + simpl in *.
+      Intros pl_head pr_head.
+      Check (IHb1 z z0 b1 b2 head pl_head pl_head pr_head).
+      sep_apply (IHb1 k' v' l' r' curr pl_head pl pr).
+      sep_apply IHb1.
+
+      destruct l'.
+      *  *)
+
+ 
+Theorem hole_rep_fuse_left : forall b k curr_k v l r (curr head pl pr: val),
+  well_ordered b ->
+  search_path k b (node (curr_k, v) l r) ->
+  k < curr_k ->
+  (node (curr_k, v) l r = b -> curr = head) ->
+    bst_hole_rep (bst_subtract_path k b (node (curr_k, v) l r)) head *
+    malloc_token Ews t_bst curr *
+    data_at Ews t_bst (Vint (Int.repr curr_k), (Vint (Int.repr v), (pl, pr))) curr *
+    bst_rep r pr
+    |-- bst_hole_rep (bst_subtract_path k b l) head.
+Proof.
+  intros.
+  generalize dependent head.
+  induction b; intros.
+  - inversion H0.
+  - simpl. destruct_pair.
+    find_Z_compare_destruct.
+    + apply search_path_is_subtree in H0.
+      apply wo_node_eq in H0; [|assumption].
+      inversion H0; subst; clear H0.
+      simplify_assumps; subst.
+      destruct l.
+      * simpl.
+        rewrite Zaux.Zcompare_Lt by assumption.
+        simpl.
+        Exists pl pr.
+        entailer!.
+      * simpl.
+        destruct_pair. 
+        rewrite Z.compare_refl.
+        rewrite Zaux.Zcompare_Lt.
+        -- simpl.
+           Exists pl pr.
+           entailer!.
+        -- inversion H; subst.
+           inversion H5; subst.
+           simpl in *; assumption.
+    + simpl in *.
+      Intros head_pl head_pr.
+      sep_apply IHb1.
+      * inversion H. assumption.
+      * inversion H0; subst.
+        -- lia.
+        -- assumption.
+        -- apply search_path_is_subtree in H10.
+           inversion H; subst.
+           eapply subtree_forall in H10; [|eapply H9].
+           inversion H10; subst.
+           simpl in *.
+           lia.
+      * admit.
+      * destruct l.
+        -- simpl. 
+           rewrite Zaux.Zcompare_Lt.
+           ++ simpl.
+              Exists head_pl head_pr.
+              entailer!.
+           ++ inversion H0; subst.
+              ** lia.
+              ** assumption.
+              ** apply search_path_is_subtree in H10.
+                 inversion H; subst.
+                 eapply subtree_forall in H10; [|eassumption].
+                 inversion H10; subst.
+                 simpl in *.
+                 lia.
+        -- simpl.
+           destruct_pair.
+           rewrite Zaux.Zcompare_Lt.
+           ++ simpl.
+              Exists head_pl head_pr.
+              entailer!.
+           ++ apply search_path_is_subtree in H0.
+              apply wo_subtree_left in H0; try assumption.
+              apply is_subtree_up_left in H0.
+              inversion H; subst.
+              eapply subtree_forall in H0; [|eassumption].
+              inversion H0; subst.
+              simpl in *; assumption.
+    + simpl in *.
+      Intros head_pl head_pr.
+      sep_apply IHb2.
+      * inversion H. assumption.
+      * inversion H0; subst.
+        -- lia.
+        -- apply search_path_is_subtree in H10.
+           inversion H; subst.
+           eapply subtree_forall in H10; [|eassumption].
+           inversion H10; subst.
+           simpl in *.
+           lia.
+        -- assumption.
+      * admit.
+      * destruct l.
+        -- simpl. 
+           rewrite Zaux.Zcompare_Gt.
+           ++ simpl.
+              Exists head_pl head_pr.
+              entailer!.
+           ++ inversion H0; subst.
+              ** lia.
+              ** apply search_path_is_subtree in H10.
+                 inversion H; subst.
+                 eapply subtree_forall in H10; [|eassumption].
+                 inversion H10; subst.
+                 simpl in *.
+                 lia.
+              ** lia.
+        -- simpl.
+           destruct_pair.
+           rewrite Zaux.Zcompare_Gt.
+           ++ simpl.
+              Exists head_pl head_pr.
+              entailer!.
+           ++ apply search_path_is_subtree in H0.
+              apply wo_subtree_right in H0; try assumption.
+              apply is_subtree_up_left in H0.
+              inversion H; subst.
+              eapply subtree_forall in H0; [|eassumption].
+              inversion H0; subst.
+              simpl in *; lia.
+Admitted.
+
+Theorem hole_rep_fuse_right : forall b k curr_k v l r (curr head pl pr: val),
+  well_ordered b ->
+  search_path k b (node (curr_k, v) l r) ->
+  k > curr_k ->
+  (node (curr_k, v) l r = b -> curr = head) ->
+    bst_hole_rep (bst_subtract_path k b (node (curr_k, v) l r)) head *
+    malloc_token Ews t_bst curr *
+    data_at Ews t_bst (Vint (Int.repr curr_k), (Vint (Int.repr v), (pl, pr))) curr *
+    bst_rep l pl
+    |-- bst_hole_rep (bst_subtract_path k b r) head.
+Proof.
+  intros.
+  generalize dependent head.
+  induction b; intros.
+  - inversion H0.
+  - simpl. destruct_pair.
+    find_Z_compare_destruct.
+    + apply search_path_is_subtree in H0.
+      apply wo_node_eq in H0; [|assumption].
+      inversion H0; subst; clear H0.
+      simplify_assumps; subst.
+      destruct r.
+      * simpl.
+        rewrite Zaux.Zcompare_Gt by lia.
+        simpl.
+        Exists pl pr.
+        entailer!.
+      * simpl.
+        destruct_pair. 
+        rewrite Z.compare_refl.
+        rewrite Zaux.Zcompare_Gt.
+        -- simpl.
+           Exists pl pr.
+           entailer!.
+        -- inversion H; subst.
+           inversion H6; subst.
+           simpl in *; lia.
+    + simpl in *.
+      Intros head_pl head_pr.
+      sep_apply IHb1.
+      * inversion H. assumption.
+      * inversion H0; subst.
+        -- lia.
+        -- assumption.
+        -- apply search_path_is_subtree in H10.
+           inversion H; subst.
+           eapply subtree_forall in H10; [|eapply H9].
+           inversion H10; subst.
+           simpl in *.
+           lia.
+      * admit.
+      * destruct r.
+        -- simpl. 
+           rewrite Zaux.Zcompare_Lt.
+           ++ simpl.
+              Exists head_pl head_pr.
+              entailer!.
+           ++ inversion H0; subst.
+              ** lia.
+              ** assumption.
+              ** apply search_path_is_subtree in H10.
+                 inversion H; subst.
+                 eapply subtree_forall in H10; [|eassumption].
+                 inversion H10; subst.
+                 simpl in *.
+                 lia.
+        -- simpl.
+           destruct_pair.
+           rewrite Zaux.Zcompare_Lt.
+           ++ simpl.
+              Exists head_pl head_pr.
+              entailer!.
+           ++ 
+              (* Show that node_z1 is a subtree of b1 *)
+              apply search_path_is_subtree in H0.
+              apply wo_subtree_left in H0; try assumption.
+              apply is_subtree_up_right in H0.
+              inversion H; subst.
+              eapply subtree_forall in H0; [|eassumption].
+              inversion H0; subst.
+              simpl in *; assumption.
+    + simpl in *.
+      Intros head_pl head_pr.
+      sep_apply IHb2.
+      * inversion H. assumption.
+      * inversion H0; subst.
+        -- lia.
+        -- apply search_path_is_subtree in H10.
+           inversion H; subst.
+           eapply subtree_forall in H10; [|eassumption].
+           inversion H10; subst.
+           simpl in *.
+           lia.
+        -- assumption.
+      * admit.
+      * destruct r.
+        -- simpl. 
+           rewrite Zaux.Zcompare_Gt.
+           ++ simpl.
+              Exists head_pl head_pr.
+              entailer!.
+           ++ inversion H0; subst.
+              ** lia.
+              ** apply search_path_is_subtree in H10.
+                 inversion H; subst.
+                 eapply subtree_forall in H10; [|eassumption].
+                 inversion H10; subst.
+                 simpl in *.
+                 lia.
+              ** lia.
+        -- simpl.
+           destruct_pair.
+           rewrite Zaux.Zcompare_Gt.
+           ++ simpl.
+              Exists head_pl head_pr.
+              entailer!.
+           ++ apply search_path_is_subtree in H0.
+              apply wo_subtree_right in H0; try assumption.
+              apply is_subtree_up_right in H0.
+              inversion H; subst.
+              eapply subtree_forall in H0; [|eassumption].
+              inversion H0; subst.
+              simpl in *; lia.
+Admitted.
+
+Lemma no_infinite_node_left {A} : forall (a: A) l r,
+  node a l r <> l.
+Proof.
+  unfold not.
+  intros.
+  induction l.
+  - discriminate.
+  - apply IHl1.
+    inversion H.
+    rewrite H2 at 1.
+    reflexivity.
+Qed.
+
+Lemma no_infinite_node_right {A} : forall (a: A) l r,
+  node a l r <> r.
+Proof.
+  unfold not.
+  intros.
+  induction r.
+  - discriminate.
+  - apply IHr2.
+    inversion H.
+    rewrite H3 at 1.
+    reflexivity.
+Qed.
+
+Fixpoint depth {A} (b: bin_tree A) : nat := 
+  match b with 
+  | leaf => 0
+  | node a l r => S (max (depth l) (depth r))
+  end.
+
+Theorem subtree_depth_monotonic {A} : forall (b1 b2: bin_tree A),
+  is_subtree b1 b2 -> (depth b1 <= depth b2)%nat.
+Proof.
+  intros.
+  dependent induction H; simpl; lia.
+Qed.
+
+Theorem no_subtree_cycle_left {A} : forall (a: A) l r,
+  not (is_subtree (node a l r) l).
+Proof.
+  unfold not.
+  intros.
+  apply subtree_depth_monotonic in H.
+  simpl in H.
+  lia.
+Qed.
+
+Theorem no_subtree_cycle_right {A} : forall (a: A) l r,
+  not (is_subtree (node a l r) r).
+Proof.
+  unfold not.
+  intros.
+  apply subtree_depth_monotonic in H.
+  simpl in H.
+  lia.
+Qed.
+
 Theorem body_search_bst: semax_body Vprog Gprog f_search_bst search_bst_spec.
 Proof.
   start_function.
   forward_loop (
-    EX curr: val, EX curr_b: bst Z, EX b_hole,
-      PROP (search_path k b curr_b)
+    EX curr_b curr,
+      PROP (search_path k b curr_b; curr_b = b -> curr = head)
       LOCAL (
         gvars gv; temp _bst__1 curr;
         temp _key (Vint (Int.repr k)))
-      SEP (b_hole; bst_rep curr_b curr; mem_mgr gv)
+      SEP (
+        bst_hole_rep (bst_subtract_path k b curr_b) head;
+        bst_rep curr_b curr; mem_mgr gv)
   ).
-  { repeat EExists.
-    entailer!.
-    - constructor.
-    - repeat entailer!. }
-  Intros curr curr_b b_hole.
-  forward_if.
-  { forward.
+  {
     repeat EExists.
     entailer!.
+    - constructor.
+    - rewrite bst_subtract_path_b_b.
+      entailer!.
+  }
+  Intros curr_b curr.
+  forward_if.
+  {
+    forward.
     simplify_assumps; subst.
     rewrite search_path_fail by assumption.
-    expand bst_rep.
-    repeat entailer!. }
+    EExists.
+    entailer!.
+    simpl.
+    entailer!.
+  }
   assert_PROP (curr_b <> leaf) by (expand bst_rep; entailer!; find_contradiction). 
-  destruct curr_b; [contradiction|].
+  destruct curr_b as [|[curr_k v] l r]; [contradiction|].
   expand bst_rep.
-  destruct_pair.
   Intros pl pr.
   forward.
   forward_if.
-  { forward.
-    erewrite search_path_constant by eassumption.
-    simpl.
-    assert (k = z).
+  {
+    assert (k = curr_k).
     { apply repr_inj_signed; try assumption.
-      apply search_path_is_subtree in H1.
-      pose proof (subtree_forall _ _ _ H1 H0) as H10.
-      inversion H10; simpl in *; assumption. }
+      apply search_path_is_subtree in H2.
+      pose proof (subtree_forall _ _ _ H2 H0) as H11.
+      inversion H11; simpl in *; assumption. }
     subst.
-    rewrite Z.compare_refl.
-    expand bst_rep.
+    forward.
     EExists.
-    Exists b_hole.
+    simpl.
     entailer!.
-    repeat EExists.
-    entailer!. }
+    erewrite search_path_success by eassumption.
+    sep_apply generalize_node_rep.
+    cancel.
+  }
   forward.
   forward_if.
-  - forward.
-    Exists pl curr_b1
-      ((b_hole * malloc_token Ews t_bst curr * 
-        data_at Ews t_bst (Vint (Int.repr z), (Vint (Int.repr z0), (pl, pr))) curr *
-        bst_rep curr_b2 pr)%logic).
+  - assert (k < curr_k).
+    {
+      rewrite <- Int.signed_repr.
+      - assumption.
+      - apply search_path_is_subtree in H2.
+        eapply subtree_forall in H2; [|eassumption].
+        inversion H2; subst.
+        simpl in H11; assumption.
+    }
+    forward.
+    Exists l pl.
     entailer!.
-    eapply path_step_down_l; [eassumption|].
-    rewrite Int.signed_repr in H5. assumption.
-    apply search_path_is_subtree in H1.
-    pose proof (subtree_forall _ _ _ H1 H0) as H11.
-    inversion H11; simpl in *; assumption.
-  - forward.
-    Exists pr curr_b2
-      ((b_hole * malloc_token Ews t_bst curr * 
-        data_at Ews t_bst (Vint (Int.repr z), (Vint (Int.repr z0), (pl, pr))) curr *
-        bst_rep curr_b1 pl)%logic).
+    + split.
+      * eapply path_step_down_l; eassumption.
+      * intro; subst.
+        apply search_path_is_subtree in H2.
+        apply no_subtree_cycle_left in H2.
+        contradiction.
+    + apply hole_rep_fuse_left; assumption.
+  - assert (k > curr_k).
+    {
+      apply search_path_is_subtree in H2.
+      pose proof (subtree_forall _ _ _ H2 H0) as H8.
+      rewrite Int.signed_repr in H7.
+      + enough (k <> curr_k). lia.
+        apply repr_inj_signed'; try assumption.
+        inversion H8; simpl in *; assumption.
+      + inversion H8; simpl in *; assumption.
+    }
+    forward.
+    Exists r pr.
     entailer!.
-    eapply path_step_down_r; [eassumption|].
-    apply search_path_is_subtree in H1.
-    pose proof (subtree_forall _ _ _ H1 H0) as H11.
-    rewrite Int.signed_repr in H5.
-    + enough (k <> z). lia.
-      apply repr_inj_signed'; try assumption.
-      inversion H11; simpl in *; assumption.
-    + inversion H11; simpl in *; assumption.
+    + split.
+      * eapply path_step_down_r; [eassumption|lia].
+      * intro; subst.
+        apply search_path_is_subtree in H2.
+        apply no_subtree_cycle_right in H2.
+        contradiction.
+    + apply hole_rep_fuse_right; assumption.
 Qed.
+
+Definition ptr_to_bst_rep b p := EX q, data_at Ews (tptr t_bst) q p * bst_rep b q.
+
+Theorem generalize_ptr_to_node_rep : forall b p q,
+  data_at Ews (tptr t_bst) q p * bst_rep b q |-- ptr_to_bst_rep b p.
+Proof.
+  intros.
+  unfold ptr_to_bst_rep.
+  EExists.
+  entailer!.
+Qed.
+
+(* Definition bst_hole_ptr_rep b p :=
+  match b with
+  | hole => emp
+  | _ => EX q, data_at Ews (tptr t_bst) q p * bst_hole_rep b q
+  end. *)
+Print bst_hole_rep.
+Fixpoint ptr_to_bst_hole_rep b p := 
+  match b with 
+  | hole => emp
+  | node_hole_l (k,v) l r =>
+      EX (q pr: val),
+        data_at Ews (tptr t_bst) q p *
+        malloc_token Ews t_bst q *
+        field_at Ews t_bst [StructField _key] (Vint (Int.repr k)) q *
+        field_at Ews t_bst [StructField _val] (Vint (Int.repr v)) q *
+        field_at Ews t_bst [StructField _right] pr q *
+        ptr_to_bst_hole_rep l (field_address t_bst [StructField _left] q) *
+        bst_rep r pr
+  | node_hole_r (k,v) l r =>
+      EX (q pl: val),
+        data_at Ews (tptr t_bst) q p *
+        malloc_token Ews t_bst q *
+        field_at Ews t_bst [StructField _key] (Vint (Int.repr k)) q *
+        field_at Ews t_bst [StructField _val] (Vint (Int.repr v)) q *
+        field_at Ews t_bst [StructField _left] pl q *
+        bst_rep l pl *
+        ptr_to_bst_hole_rep r (field_address t_bst [StructField _right] q)
+  end.
+
+Theorem body_insert_bst: semax_body Vprog Gprog f_insert_bst insert_bst_spec.
+Proof.
+  start_function.
+  forward_loop (
+    EX curr_b curr_ptr,
+      PROP (
+        search_path k b curr_b;
+        curr_b = b -> curr_ptr = bst_ptr)
+      LOCAL (
+        gvars gv; temp _bst__1 curr_ptr;
+        temp _key (Vint (Int.repr k));
+        temp _val (Vint (Int.repr v)))
+      SEP (
+        ptr_to_bst_hole_rep (bst_subtract_path k b curr_b) bst_ptr;
+        ptr_to_bst_rep curr_b curr_ptr;
+        mem_mgr gv)
+  ).
+  {
+    Exists b bst_ptr.
+    entailer!.
+    - constructor.
+    - rewrite bst_subtract_path_b_b.
+      simpl. cancel.
+      unfold ptr_to_bst_rep.
+      Exists head.
+      entailer!.
+  }
+  unfold ptr_to_bst_rep.
+  Intros curr_b curr_ptr curr.
+  forward.
+  forward_if.
+  {
+    subst.
+    forward_call.
+    Intros vret.
+    repeat forward.
+    simplify_assumps; subst.
+    simpl bst_rep at 2; entailer!.
+
+    revert H3 H4.
+    clear.
+    generalize dependent bst_ptr.
+    induction b; intros.
+    - simpl.
+      simplify_assumps; subst.
+      Intros pl pr.
+      Exists vret pl pr.
+      entailer!.
+    - clear H4.
+      simpl bst_subtract_path.
+      destruct_pair.
+      find_Z_compare_destruct.
+      + apply search_path_fail in H3.
+        simpl in H3.
+        rewrite Z.compare_refl in H3.
+        discriminate H3.
+      + simpl bst_subtract_path in *.
+        simpl ptr_to_bst_hole_rep.
+        Intros q pr.
+        (* sep_apply (IHb1 (field_address t_bst [StructField _left] q)). *)
+        sep_apply IHb1.
+        * inversion H3; subst; [assumption | lia].
+        * admit.
+        * Intros a.
+          Exists q.
+          entailer!.
+          simpl.
+          rewrite Zaux.Zcompare_Lt by assumption.
+          simpl.
+          Exists a pr.
+          entailer!.
+          unfold_data_at (data_at _ _ _ q).
+          entailer!.
+      + simpl bst_subtract_path in *.
+        simpl ptr_to_bst_hole_rep.
+        Intros q pl.
+        (* sep_apply (IHb2 (field_address t_bst [StructField _right] q)). *)
+        sep_apply IHb2.
+        * inversion H3; subst; [lia | assumption].
+        * admit.
+        * Intros a.
+          Exists q.
+          entailer!.
+          simpl.
+          rewrite Zaux.Zcompare_Gt by lia.
+          simpl.
+          Exists pl a.
+          entailer!.
+          unfold_data_at (data_at _ _ _ q).
+          entailer!.
+  }
+  assert_PROP (curr_b <> leaf) by (expand bst_rep; entailer!; find_contradiction). 
+  destruct curr_b as [|[curr_k curr_v] l r]; [contradiction|].
+  expand bst_rep.
+  Intros pl pr.
+  repeat forward.
+  forward_if.
+  {
+    repeat forward.
+    assert (k = curr_k).
+    { apply repr_inj_signed; try assumption.
+      apply search_path_is_subtree in H3.
+      eapply subtree_forall in H3; [|eassumption].
+      inversion H3; simpl in *; assumption. }
+    subst.
+    simpl.
+    sep_apply generalize_node_rep.
+    sep_apply generalize_ptr_to_node_rep.
+
+    assert ((
+      ptr_to_bst_rep (insert curr_k v b) bst_ptr * mem_mgr gv
+      =
+      EX a : val,
+      data_at Ews (tptr t_bst) a bst_ptr *
+      (bst_rep (insert curr_k v b) a * mem_mgr gv)
+    )%logic).
+    { apply pred_ext; unfold ptr_to_bst_rep; Intros q; Exists q; entailer!. }
+    rewrite <- H15.
+    entailer!.
+
+    revert H2 H3 H4.   
+    clear.
+    revert bst_ptr.
+    induction b; intros.
+    - inversion H3.
+    - simpl.
+      destruct_pair.
+      find_Z_compare_destruct.
+      + simpl; cancel.
+        apply search_path_is_subtree in H3.
+        apply wo_node_eq in H3; [|assumption].
+        inversion H3; subst.
+        simplify_assumps; subst.
+        entailer!.
+      + simpl.
+        Intros q pr.
+        sep_apply IHb1.
+        * inversion H2; assumption.
+        * inversion H3; subst; lia + assumption.
+        * admit.
+        * unfold ptr_to_bst_rep.
+          Intros pl.
+          Exists q.
+          entailer!.
+          simpl.
+          Exists pl pr.
+          unfold_data_at (data_at _ _ _ q).
+          entailer!.
+      + simpl.
+        Intros q pl.
+        sep_apply IHb2.
+        * inversion H2; assumption.
+        * inversion H3; subst; lia + assumption.
+        * admit.
+        * unfold ptr_to_bst_rep.
+          Intros pr.
+          Exists q.
+          entailer!.
+          simpl.
+          Exists pl pr.
+          unfold_data_at (data_at _ _ _ q).
+          entailer!.
+  }
+  repeat forward.
+  forward_if.
+  {
+    assert (k < curr_k).
+    {
+      rewrite <- Int.signed_repr.
+      - assumption.
+      - apply search_path_is_subtree in H3.
+        eapply subtree_forall in H3; [|eassumption].
+        inversion H3; subst.
+        simpl in *; assumption.
+    }
+    repeat forward.
+    simpl offset_val.
+    entailer!.
+    Exists l (field_address t_bst [StructField _left] curr).
+    entailer!.
+    - split.
+      + eapply path_step_down_l; eassumption.
+      + intro; subst.
+        apply search_path_is_subtree in H3.
+        apply no_subtree_cycle_left in H3.
+        contradiction.
+    - sep_apply generalize_node_rep.
+      simpl bst_subtract_path.
+      revert bst_ptr H2 H3 H4.   
+      clear - H9.
+      induction b; intros; [inversion H3|].
+      simpl.
+      Intros pl pr.
+      destruct_pair.
+      find_Z_compare_destruct.
+      + apply search_path_is_subtree in H3.
+        apply wo_node_eq in H3; [|assumption].
+        inversion H3; subst.
+        simplify_assumps; subst.
+        destruct l.
+        * simpl.
+          rewrite Zaux.Zcompare_Lt by assumption.
+          simpl.
+          unfold ptr_to_bst_rep.
+          Exists curr pr pl.
+          expand bst_rep.
+          unfold_data_at (data_at _ _ _ curr).
+          entailer!.
+        * simpl.
+          destruct_pair.
+          Intros pl' pr'.
+          rewrite Z.compare_refl.
+          rewrite Zaux.Zcompare_Lt.
+          -- simpl.
+             unfold ptr_to_bst_rep.
+             Exists curr pr pl.
+             unfold_data_at (data_at _ _ _ curr).
+             entailer!.
+             apply generalize_node_rep.
+          -- inversion H2; subst.
+             inversion H4; subst.
+             simpl in H3; assumption.
+      + simpl.
+        Intros q pr'.
+        sep_apply generalize_node_rep.
+        sep_apply IHb1.
+        * inversion H2; assumption.
+        * inversion H3; lia + assumption.
+        * admit.
+        * entailer!.
+          destruct l.
+          -- simpl.
+             rewrite Zaux.Zcompare_Lt.
+             ++ simpl.
+                Exists q pr'.
+                entailer!.
+             ++ inversion H3; lia.
+          -- simpl.
+             destruct_pair.
+             rewrite Zaux.Zcompare_Lt.
+             ++ simpl.
+                Exists q pr'.
+                entailer!.
+             ++ inversion H3; subst; try lia.
+                apply search_path_is_subtree in H20.
+                apply subtree_well_ordered in H20; [|inversion H2; assumption].
+                inversion H20; subst.
+                inversion H18; subst.
+                simpl in H17; lia.
+      + simpl.
+        Intros q pl'.
+        sep_apply generalize_node_rep.
+        sep_apply IHb2.
+        * inversion H2; assumption.
+        * inversion H3; subst.
+          -- lia.
+          -- apply search_path_is_subtree in H10.
+             eapply subtree_forall in H10; [| inversion H2; eassumption].
+             inversion H10; subst.
+             simpl in H6; lia.
+          -- assumption.
+        * admit.
+        * cancel.
+          destruct l.
+          -- simpl.
+             rewrite Zaux.Zcompare_Gt.
+             ++ simpl.
+                Exists q pl'.
+                entailer!.
+             ++ inversion H3; subst; try lia.
+                apply search_path_is_subtree in H10.
+                eapply subtree_forall in H10; [| inversion H2; eassumption].
+                inversion H10; subst.
+                simpl in H6; lia.
+          -- simpl.
+             destruct_pair.
+             rewrite Zaux.Zcompare_Gt.
+             ++ simpl.
+                Exists q pl'.
+                entailer!.
+             ++ apply search_path_is_subtree in H3.
+                apply wo_subtree_right in H3; [|assumption|lia].
+                apply is_subtree_up_left in H3.
+                eapply subtree_forall in H3; [|inversion H2; eassumption].
+                inversion H3; subst.
+                simpl in H6; lia.
+  }
+  {
+    assert (k > curr_k).
+    {
+      apply search_path_is_subtree in H3.
+      eapply subtree_forall in H3; [|eassumption].
+      rewrite Int.signed_repr in H8.
+      + enough (k <> curr_k). lia.
+        apply repr_inj_signed'; try assumption.
+        inversion H3; simpl in *; assumption.
+      + inversion H3; simpl in *; assumption.
+    }
+    repeat forward.
+    simpl offset_val.
+    entailer!.
+    Exists r (field_address t_bst [StructField _right] curr).
+    entailer!.
+    - split.
+      + eapply path_step_down_r; eassumption + lia.
+      + intro; subst.
+        apply search_path_is_subtree in H3.
+        apply no_subtree_cycle_right in H3.
+        contradiction.
+    - sep_apply generalize_node_rep.
+      simpl bst_subtract_path.
+      revert bst_ptr H2 H3 H4.   
+      clear - H9.
+      induction b; intros; [inversion H3|].
+      simpl.
+      Intros pl pr.
+      destruct_pair.
+      find_Z_compare_destruct.
+      + apply search_path_is_subtree in H3.
+        apply wo_node_eq in H3; [|assumption].
+        inversion H3; subst.
+        simplify_assumps; subst.
+        destruct r.
+        * simpl.
+          rewrite Zaux.Zcompare_Gt by lia.
+          simpl.
+          unfold ptr_to_bst_rep.
+          Exists curr pl pr.
+          expand bst_rep.
+          unfold_data_at (data_at _ _ _ curr).
+          entailer!.
+        * simpl.
+          destruct_pair.
+          Intros pl' pr'.
+          rewrite Z.compare_refl.
+          rewrite Zaux.Zcompare_Gt.
+          -- simpl.
+             unfold ptr_to_bst_rep.
+             Exists curr pl pr.
+             unfold_data_at (data_at _ _ _ curr).
+             entailer!.
+             apply generalize_node_rep.
+          -- inversion H2; subst.
+             inversion H5; subst.
+             simpl in H3; lia.
+      + simpl.
+        Intros q pr'.
+        sep_apply generalize_node_rep.
+        sep_apply IHb1.
+        * inversion H2; assumption.
+        * inversion H3; subst.
+          -- lia.
+          -- assumption.
+          -- apply search_path_is_subtree in H10.
+             eapply subtree_forall in H10; [| inversion H2; eassumption].
+             inversion H10; subst.
+             simpl in H6; lia.
+        * admit.
+        * cancel.
+          destruct r.
+          -- simpl.
+             rewrite Zaux.Zcompare_Lt.
+             ++ simpl.
+                Exists q pr'.
+                entailer!.
+             ++ inversion H3; subst.
+                ** lia.
+                ** assumption.   
+                ** apply search_path_is_subtree in H10.
+                   eapply subtree_forall in H10; [| inversion H2; eassumption].
+                   inversion H10; subst.
+                   simpl in H6; lia.
+          -- simpl.
+             destruct_pair.
+             rewrite Zaux.Zcompare_Lt.
+             ++ simpl.
+                Exists q pr'.
+                entailer!.
+             ++ inversion H3; subst.
+                ** lia.
+                ** apply search_path_is_subtree in H10.
+                   apply is_subtree_up_right in H10.
+                   eapply subtree_forall in H10; [| inversion H2; eassumption].
+                   inversion H10; subst.
+                   simpl in H6; lia.
+                ** apply search_path_is_subtree in H10.
+                   eapply subtree_forall in H10; [| inversion H2; eassumption].
+                   inversion H10; subst.
+                   simpl in H6; lia.
+      + simpl.
+        Intros q pl'.
+        sep_apply generalize_node_rep.
+        sep_apply IHb2.
+        * inversion H2; assumption.
+        * inversion H3; subst.
+          -- lia.
+          -- apply search_path_is_subtree in H10.
+             eapply subtree_forall in H10; [| inversion H2; eassumption].
+             inversion H10; subst.
+             simpl in H6; lia.
+          -- assumption.
+        * admit.
+        * cancel.
+          destruct r.
+          -- simpl.
+             rewrite Zaux.Zcompare_Gt.
+             ++ simpl.
+                Exists q pl'.
+                entailer!.
+             ++ inversion H3; lia.
+          -- simpl.
+             destruct_pair.
+             rewrite Zaux.Zcompare_Gt.
+             ++ simpl.
+                Exists q pl'.
+                entailer!.
+             ++ apply search_path_is_subtree in H3.
+                apply wo_subtree_right in H3; [|assumption|lia].
+                apply is_subtree_up_right in H3.
+                eapply subtree_forall in H3; [|inversion H2; eassumption].
+                inversion H3; subst.
+                simpl in H6; lia.
+  }
+Admitted.
